

* Linear Regression

Linear Regression \rightarrow method to find straight-line relationship b/w input (X) & output (Y).

\hookrightarrow If X changes, how does Y change

* It is used only when

\hookrightarrow output is continuous value

\hookrightarrow Dataset must be linear in nature

i.e. Relationship b/w X & Y is straight line.

$y = mx + c$ \rightarrow eqⁿ of straight line
in ml,

$$\hat{y} = \beta_0 + \beta_1 x$$

$x \rightarrow$ input feature

$\hat{y} \rightarrow y$ - predicted \rightarrow output

$\beta_0 \rightarrow$ intercept \rightarrow value of y at $x=0$.

$\beta_1 \rightarrow$ slope / weight

* How it works

Tries many possible lines and measures error and continue doing till error converges and picks the line with minimum error.

* Loss function / Cost function \rightarrow to measure total error, here we use MSE (Mean squared error).

$$\left\{ \text{MSE} = \frac{1}{n} \sum (y - \hat{y})^2 \right\}$$

\downarrow \downarrow
 Actual Predicted

* Two types

\hookrightarrow simple LR \rightarrow one input feature $[\hat{y} = \beta_0 + \beta_1 x]$

\hookrightarrow Multiple LR \rightarrow More than one feature $[\hat{y} = \beta_0 + \beta_1 x_1 + \beta_2 x_2 + \dots]$

- * Evaluation metric \rightarrow MSE \rightarrow mean squared error
 R^2 score \rightarrow goodness of fit (0 to 1)
 0 \rightarrow model explain nothing
 1 \rightarrow perfect fit.

* When to use

- Relationship is linear (can be increasing / decreasing)
 can't be curved / random
- Output is continuous

* Avoid when

- Data is highly non-linear
- Many outliers
- Classification problem.

$$\left. \begin{array}{l} \text{Prediction} \\ \uparrow \\ \hat{y} = \underbrace{\beta_0}_{\text{Bias}} + \underbrace{\beta_1 x_1}_{\text{Weight}} \end{array} \right\} \begin{array}{l} \text{input} \\ \text{Feature} \end{array}$$

\downarrow
trainable

- * Mostly training in LR follow Gradient Descent method.

idea

- \hookrightarrow Start with random value of β
- \hookrightarrow Move step by step toward min error
- \hookrightarrow Stop when improvement is very small.

$$\text{Update formula} \rightarrow \theta = \theta - \alpha \frac{\partial J}{\partial \theta}$$

$$\left[\begin{array}{l} \alpha \rightarrow \text{learning rate} \\ J \rightarrow \text{Cost function} \end{array} \right] \alpha \text{ or } \eta$$

both are learning rate symbol

Example \rightarrow Properly random ^{simple} example just to understand functioning.

x	y
1	5
2	7
3	9
4	11

$$\hat{y} = mx + c$$

taking $m = 0$, $c = 0$ (trainable).

calculate \hat{y} with x as 1, 2, 3, 4

$$\hat{y} = 0$$

Calculate error,

$$MSE = \frac{1}{4} [(5-0)^2 + (7-0)^2 + (9-0)^2 + (11-0)^2]$$

$$= 69 \rightarrow \text{loss}$$

now, we will update both m & c (trainable parameter) by gradient descent.

$$m_n = m_o - \eta \frac{\partial MSE}{\partial m} \quad \text{①} \quad \left\{ \begin{array}{l} \text{Formula} \\ \theta = \theta - \eta \frac{\partial \text{cost func}}{\partial \theta} \end{array} \right.$$

\downarrow \downarrow
 m_{new} m_{old}

$$c_n = c_o - \eta \frac{\partial MSE}{\partial c} \quad \text{②}$$

$$MSE = \frac{1}{n} \sum_{i=1}^n (y_i - \hat{y})^2$$

$$= \frac{1}{n} \sum (y - (mx_i + c))^2 \quad (\hat{y} = mx + c)$$

$$\text{Put } y - (mx_i + c) = E$$

$$= \frac{1}{n} \sum (E)^2$$

now partial derivative of MSE with m .

$$\frac{\partial MSE}{\partial m} = \frac{1}{n} \sum 2E \left(\frac{\partial E}{\partial m} \right)$$

$$= \frac{1}{n} \sum 2E (-x)$$

$$= \frac{1}{n} \sum 2(y - (mx + c))(-x)$$

$$\left\{ \begin{array}{l} \frac{\partial E}{\partial m} = \frac{\partial (y - (mx + c))}{\partial m} \\ = \frac{\partial (y - mx + c)}{\partial m} \\ = -x \end{array} \right.$$

$$= -x$$

$$= -x$$

$$= \frac{1}{n} \sum (2y - 2mx - 2c)(-x)$$

$$= \frac{1}{n} \sum (-2yx + 2mx^2 + 2xc)$$

$$= \frac{-2x \sum (y - mx - c)}{n}$$

$$= \frac{-2x \sum (y - (mx + c))}{n}$$

$$\frac{\partial \text{MSE}}{\partial m} = \frac{-2}{n} \sum x (y - \hat{y})$$

Put in (1)

$$m_n = m_0 - \eta \frac{\partial \text{MSE}}{\partial m}$$

$$\bullet \left\{ m_n = m_0 - \eta \left(\frac{-2}{n} \sum x (y - \hat{y}) \right) \right\}$$

calculate new m

$$m_n = 0 - 0.1 \left(\frac{-2}{4} [1(5-0) + 2(7-0) + 3(9-0) + 4(11-0)] \right)$$

$$= 4.5$$

• Like that we will find $c_n = c_0 - \eta \frac{\partial \text{MSE}}{\partial c}$

Similarly, c_n will come out like solve as we solve for m_n .

$$\frac{\partial \text{MSE}}{\partial c} = \frac{-2}{n} \sum (y - \hat{y})$$

$$c_n = c_0 - \eta \frac{\partial \text{MSE}}{\partial c}$$

$$c_n = c_0 - \eta \left(\frac{-2}{n} \sum (y - \hat{y}) \right)$$

$$\bullet \left\{ c_n = c_0 + \eta \left(\frac{2}{n} \sum (y - \hat{y}) \right) \right\}$$

$$C_n = 0 + 0.1 \left(\frac{2}{4} (5-0 + 7-0 + 9-0 + 11-0) \right)$$

$$C_n = 1.6$$

We got $m_n = 4.5$, $C_n = 1.6$

$$eq^n = \hat{y} = 4.5x + 1.6$$

x	y	\hat{y}	By using new eq ⁿ
1	5	6.1	
2	7	10.6	Again calculate Loss
3	9	15.1	MSE = $\frac{1}{n} \sum (y - \hat{y})^2$
4	11	19.6	

$$= \frac{1}{4} \left((5-6.1)^2 + (7-10.6)^2 + (9-15.1)^2 + (11-19.6)^2 \right)$$

$$= 31.33$$



In one iteration we

decrease loss from 69 to 31.33

Like this we this algorithm

works & keep on doing till

Loss get minimal & converge properly